pulse/src/checker/Pulse.RuntimeUtils.fsti
@@ -44,6 +44,7 @@ val embed_st_term_for_extraction (d:'a) (r:option range): T.term
 val unembed_st_term_for_extraction (d:T.term) : 'a
 val unembed_pulse_decl (d:'a) : 'b
 module R = FStar.Reflection.V2
+val push_univ_vars (g: env) (us: list R.univ_name) : g':env { g' == g }
 val debug_subst (s:list R.subst_elt) (t:T.term) (r1 r2:T.term): y:T.term{ y == r1 }
 val deep_compress (t:T.term) : r:T.term { t == r }
 (* ***WARNING*** *)
